pushing on global_extends, progress is slow

verif/GlobalExtends.v
@@ -15,12 +15,12 @@ Require Import BuiltinSyntax.
 Require Import Values.        
 Require Import Eager.
 Require Import Bitstream.
+Require Import Lib.
 
 
 Definition name_irrel {A : Type} (E : ident -> option A) : Prop :=
   forall id id',
     if ident_eq id id' then E id = E id' else True.
-
 
 Lemma name_irrel_diff_results :
   forall {A} E id id',
@@ -37,8 +37,49 @@ Proof.
   exists n. eauto.
 Qed.
 
+Definition same_values (ge GE : genv) : Prop :=
+  forall id v,
+    ge id = Some v ->
+    GE id = Some v.
 
-Definition global_extends (ge GE : genv) : Prop := True.
+Definition finite (ge : genv) : Prop :=
+  exists l,
+  forall id,
+    ge id <> None <-> In id l.
+
+Fixpoint make_ge (l : list (ident * Expr)) (ge : genv) : genv :=
+  match l with
+  | nil => ge
+  | (id,exp) :: l' =>
+    let ge' := make_ge l' ge in
+    extend ge' id exp
+  end.
+
+Definition finite' (ge : genv) (l : list (ident * Expr)) : Prop :=
+  forall id,
+    ge id = make_ge l gempty id.
+
+Fixpoint id_In (ide : (ident * Expr)) (l : list (ident * Expr)) : Prop :=
+  match l with
+  | nil => False
+  | (id,e) :: l =>
+    match ide with
+    | (id',e') => (fst id = fst id' /\ e = e') \/ id_In (id',e') l
+    end
+  end.
+
+(* lowercase is concrete, uppercase is abstract *)
+(* wf_env lets this proof be used over a variety of environments that meet the proper constraints *)
+Definition wf_env (ge GE : genv) (TE : tenv) (SE : senv)  : Prop :=
+  name_irrel ge /\ name_irrel GE /\ name_irrel TE /\ name_irrel SE /\ (*finite GE /\*)
+  (forall id,
+      ge id <> None -> (TE id = None /\ SE id = None /\ ge id = GE id)).
+
+Definition global_extends (ge GE : genv) : Prop :=
+  same_values ge GE /\
+  finite ge /\ finite GE /\
+  name_irrel ge.
+
 (* TODO *)
 (*
 Definition global_extends (ge GE : genv) : Prop :=
@@ -56,30 +97,237 @@ Definition global_extends (ge GE : genv) : Prop :=
 *)
 
 Lemma global_extends_refl :
-  forall ge,
-    global_extends ge ge.
+  forall ge GE TE SE,
+    wf_env ge GE TE SE ->
+    global_extends GE GE.
 Proof.
+  intros.
+  unfold wf_env in *.
+  repeat match goal with
+         | [ H : _ /\ _ |- _ ] => destruct H
+         end.
+  unfold global_extends. split; auto.
+  unfold same_values.
+  intros. auto.
 Admitted.
-(*
-  unfold global_extends.
-  split. auto.
-  split. auto.
-  admit. (* TODO: we'll need to pass this in *)
-Admitted.
-*)
-(*
-Lemma global_extends_eager_eval' :
-    forall expr TE SE ge GE,
-      global_extends ge GE ->
-      forall v,
-        eager_eval_expr ge TE SE expr v ->
-        eager_eval_expr GE TE SE expr v.
-Proof.
-  intros. unfold global_extends in *.
-  destruct H. destruct H1.
-  eapply H1; eauto.
-Qed.*)
 
+Lemma global_extends_extend_r :
+  forall ge ge',
+    global_extends ge ge' ->
+    forall id exp,
+      ge id = None ->
+      global_extends ge (extend ge' id exp).
+Proof.
+  intros.
+  unfold global_extends in *.
+  repeat match goal with
+         | [ H : _ /\ _ |- _ ] => destruct H
+         end.
+  split; auto; [idtac | split; auto].
+  unfold same_values in *.
+  intros.
+  destruct (ident_eq id0 id) eqn:?; auto.
+  unfold name_irrel in *. 
+  specialize (H3 id0 id). rewrite Heqs in H3.
+  congruence.
+  unfold extend.
+  rewrite Heqs.
+  eapply H; eauto.
+  split; auto.
+  
+  admit. (* finite extends to finite *)
+  
+Admitted.
+
+(*
+Inductive eager_eval_expr_listenv (ge : list (ident * Expr)) : tenv -> senv -> Expr -> strictval -> Prop :=
+| eval_bind_list :
+    forall TE SE e v,
+      eager_eval_expr (make_ge ge gempty) TE SE e v ->
+      eager_eval_expr_listenv ge TE SE e v.
+
+Lemma eval_with_list_same :
+  forall ge TE SE e v,
+    eager_eval_expr (make_ge ge gempty) TE SE e v <->
+    eager_eval_expr_listenv ge TE SE e v.
+Proof.
+  intros; split.
+  intros. econstructor; eauto.
+  intros.
+  inversion H. eauto.
+Qed.
+ *)
+
+Lemma name_irrel_extend :
+  forall {A} E id (x : A),
+    name_irrel E ->
+    name_irrel (extend E id x).
+Proof.
+  intros. unfold name_irrel in *.
+  intros.
+  specialize (H id0 id').
+  destruct (ident_eq id0 id') eqn:?; auto.
+  unfold extend.
+  destruct (ident_eq id0 id);
+    destruct (ident_eq id' id); auto.
+  rewrite e in e0. congruence.
+  rewrite e in n. congruence.
+Qed.
+
+Lemma name_irrel_erase :
+  forall {A} (E : ident -> option A) id,
+    name_irrel E ->
+    name_irrel (fun x => if ident_eq x id then None else E x).
+Proof.
+  intros.
+  unfold name_irrel in *.
+  intros.
+  specialize (H id0 id').
+  destruct (ident_eq id0 id'); auto.
+  rewrite H.
+  destruct (ident_eq id0 id);
+    destruct (ident_eq id' id);
+    auto; congruence.
+Qed.
+
+
+Lemma finite'_id_In :
+  forall l ge id exp,
+    ge id = Some exp ->
+    finite' ge l ->
+    id_In (id,exp) l.
+Proof.
+  induction l; intros;
+    unfold finite' in H0;
+    erewrite H0 in H. simpl in H. unfold gempty in *.  congruence.
+  simpl in H. destruct a.
+  unfold extend in H.
+  destruct (ident_eq id i). simpl. left. split; congruence.
+  simpl. right. eapply IHl; eauto.
+  unfold finite'. intros. reflexivity.
+Qed.
+
+
+Lemma make_ge_id_in :
+  forall l id exp,
+    make_ge l gempty id = Some exp ->
+    id_In (id,exp) l.
+Proof.
+  induction l; intros.
+  simpl in H. unfold gempty in H. congruence.
+  simpl in H. destruct a.
+  unfold extend in H. destruct (ident_eq id i).
+  simpl. left. split; congruence.
+  simpl. right.
+  eapply IHl; eauto.
+Qed.
+
+Lemma free_ge :
+  forall expr ge TE SE v,  
+    eager_eval_expr ge TE SE expr v ->
+    forall ge',
+      (forall id e, ge id = Some e ->
+                    ge' id = Some e /\
+                    forall TE SE v,
+                      eager_eval_expr ge TE SE e v ->
+                      eager_eval_expr ge' TE SE e v
+      ) ->
+      eager_eval_expr ge' TE SE expr v.
+Proof.
+  intro.
+  eapply Expr_ind_useful with (e := expr); intros.
+  Focus 8.
+  inversion H. subst.
+  econstructor; eauto.
+  subst.
+  eapply H0 in H3. destruct H3.
+  eapply H3 in H6. eapply eager_eval_global_var; eauto.
+
+  inversion H0. subst.
+  econstructor; eauto.
+  admit. admit.
+
+  inversion H0. subst.
+  econstructor; eauto.
+  unfold Pl in H.
+  eapply Forall_Forall2_implies; try eassumption.
+  intros. simpl in H2.
+  eapply H2; eauto.
+
+  (* This is true, can finish proof if needed *)
+Admitted.
+
+
+
+Lemma eager_eval_expr_from_make_ge :
+  forall expr l ge TE SE v,
+    finite' ge l ->
+    (forall id exp',
+        id_In (id,exp') l ->
+        forall v',
+          eager_eval_expr (make_ge l gempty) TE SE exp' v' ->
+          eager_eval_expr ge TE SE exp' v') ->
+    eager_eval_expr (make_ge l gempty) TE SE expr v ->
+    eager_eval_expr ge TE SE expr v.
+Proof.
+  intro.
+  eapply Expr_ind_useful with (e := expr); intros;
+    try solve [
+           try (match goal with
+                 | [ H : eager_eval_expr _ _ _ _ _ |- _ ] => inversion H; clear H
+                 end);
+          econstructor; eauto].
+  Focus 7.
+  inversion H1. subst.
+  econstructor; eauto.
+  subst. eapply eager_eval_global_var; eauto.
+  unfold finite' in *. rewrite H. eauto.
+  eapply H0; eauto.
+  eapply finite'_id_In.
+  unfold finite' in H. rewrite <- H in H4.
+  eassumption. eauto.
+
+  inversion H2. subst. econstructor; eauto.
+  (* this is provable *)
+
+  
+Admitted.
+
+
+Lemma eager_eval_expr_make_ge :
+  forall expr l ge TE SE v,
+    finite' ge l ->
+    (forall id exp',
+        id_In (id,exp') l ->
+        forall v',
+          eager_eval_expr ge TE SE exp' v' ->
+          eager_eval_expr (make_ge l gempty) TE SE exp' v') ->
+    eager_eval_expr ge TE SE expr v ->
+    eager_eval_expr (make_ge l gempty) TE SE expr v.
+Proof.
+  intro.
+  eapply Expr_ind_useful with (e := expr); intros.
+
+  unfold Pl in *. inversion H2; subst; econstructor; eauto.
+  admit. admit.
+
+  admit. admit. admit. admit.
+  admit. admit. 
+
+  subst. inversion H1; try solve [econstructor; eauto]. subst. eapply eager_eval_global_var; eauto.
+  unfold finite' in *. rewrite H in H4. eauto.
+  eapply H0; eauto.
+  instantiate (1 := id).
+  eapply finite'_id_In; eauto.
+
+  admit. admit. admit.
+  admit. admit. admit.
+
+  (* This one's true, will take a while to prove *)  
+Admitted.
+
+
+(* at the end of the day I need this fact *)
 Lemma global_extends_eager_eval :
     forall expr v ge TE SE,
       eager_eval_expr ge TE SE expr v ->
@@ -87,7 +335,75 @@ Lemma global_extends_eager_eval :
         global_extends ge GE ->
         eager_eval_expr GE TE SE expr v.
 Proof.
+  intros.
+  unfold global_extends in *.
+  repeat match goal with
+         | [ H : _ /\ _ |- _ ] => destruct H
+         end.
+  unfold finite in *.
+  destruct H1 as [l]. destruct H2 as [l'].
+  unfold same_values in *.
+  assert (forall id, In id l -> In id l').
+  intros. eapply H2.
+  destruct (ge id) eqn:?.
+  eapply H0 in Heqo. congruence.
+  erewrite <- H1 in H4. congruence.
+  
+  
+  
 Admitted.
+
+
+
+(*
+(* is this necessary? *)
+Lemma finite_make_ge :
+  forall ge,
+    finite ge ->
+    name_irrel ge ->
+    exists l,
+      forall id,
+        ge id  = make_ge l gempty id.
+Proof.
+  intros. unfold finite in *.
+  destruct H.
+  generalize dependent ge.
+  induction x; intros. exists nil.
+  simpl in H. intros.
+  destruct (ge id) eqn:?.
+  assert (ge id <> None) by congruence.
+  erewrite H in H1. inversion H1.
+  simpl. unfold gempty. reflexivity.
+
+  destruct (ge a) eqn:?.
+  Focus 2.
+  assert (In a (a :: x)) by (simpl; left; reflexivity).
+  erewrite <- H in H1. congruence.
+
+  remember (fun id => if ident_eq id a then None else ge id) as ge'.
+  assert (forall id, ge' id <> None <-> In id x). {
+    admit. (* idents ignore second part, which is hard *)
+    (* this is not quite true both ways, backwards In id x -> ge' id <> None is hard *)
+  }
+
+  eapply IHx in H1.
+  destruct H1 as [l'].
+  exists ((a,e) :: l').
+  intros.
+  simpl. unfold extend.
+  unfold name_irrel in H0.
+  specialize (H0 id a).
+  destruct (ident_eq id a) eqn:?.
+  congruence.
+  rewrite <- H1.
+  subst ge'.
+  rewrite Heqs. reflexivity.
+  subst ge'.
+  eapply name_irrel_erase; eauto.
+Admitted.
+*)
+
+
 (*  intros. eapply global_extends_eager_eval'; eauto.
 Qed.*)
 
@@ -150,15 +466,6 @@ Proof.
 Admitted.
  *)
 
-Lemma global_extends_extend_r :
-  forall ge ge',
-    global_extends ge ge' ->
-    name_irrel ge ->
-    forall id exp,
-      ge id = None ->
-      global_extends ge (extend ge' id exp).
-Proof.
-Admitted.
 (*  intros.
   unfold global_extends in *.
   destruct H. split.
