verif/Kinit_eval.v
@@ -15,6 +15,7 @@ Require Import BuiltinSyntax.
 Require Import Values.        
 Require Import Eager.
 Require Import Bitstream.
+Require Import GlobalExtends.
 
 Require Import EvalTac.
 
@@ -26,6 +27,7 @@ Require Import HMAC.
 Require Import HMAC_spec.
 
 Require Import HMAC_lib.
+
 
 
 Lemma kinit_eval :
